Rename uint and fix more style issues

src/StandardLibrary/UInt.dfy
@@ -1,130 +1,121 @@
 module {:extern "STLUInt"} StandardLibrary.UInt {
-  const UINT8_LIMIT := 0x100
-  newtype UInt8 = x | 0 <= x < UINT8_LIMIT
+  newtype uint8 = x | 0 <= x < 0x100
 
-  const UINT16_LIMIT := 0x1_0000
-  newtype UInt16 = x | 0 <= x < UINT16_LIMIT
+  newtype uint16 = x | 0 <= x < 0x1_0000
 
-  newtype Int32 = x | -0x8000_0000 <= x < 0x8000_0000
+  newtype int32 = x | -0x8000_0000 <= x < 0x8000_0000
 
-  const UINT32_LIMIT := 0x1_0000_0000
-  newtype UInt32 = x | 0 <= x < UINT32_LIMIT
+  newtype uint32 = x | 0 <= x < 0x1_0000_0000
 
-  newtype UInt64 = x | 0 <= x < 0x1_0000_0000_0000_0000
+  newtype uint64 = x | 0 <= x < 0x1_0000_0000_0000_0000
 
-  function method UInt16ToSeq(x: UInt16): seq<UInt8>
+  function method UInt16ToSeq(x: uint16): seq<uint8>
     ensures |UInt16ToSeq(x)| == 2
   {
-    var b0: UInt8 := (x / 0x100) as UInt8;
-    var b1: UInt8 := (x % 0x100) as UInt8;
+    var b0: uint8 := (x / 0x100) as uint8;
+    var b1: uint8 := (x % 0x100) as uint8;
     [b0, b1]
   }
 
-  function method SeqToUInt16(p: seq<UInt8>): UInt16
-    requires |p| == 2
+  function method SeqToUInt16(s: seq<uint8>): uint16
+    requires |s| == 2
   {
-    var x0 := (p[0] as int) * 0x100;
-    assert x0 <= UINT8_LIMIT * 0x100;
-    var x := x0 + (p[1] as int);
-    assert x < UINT16_LIMIT;
-    x as UInt16
+    var x0 := s[0] as int * 0x100;
+    var x := x0 + s[1] as int;
+    x as uint16
   }
 
-  lemma UInt16SeqSerDeser(x: UInt16)
+  lemma UInt16SeqSerDeser(x: uint16)
     ensures SeqToUInt16(UInt16ToSeq(x)) == x
   {}
 
-  lemma UInt16SeqDeserSer(s: seq<UInt8>)
+  lemma UInt16SeqDeserSer(s: seq<uint8>)
     requires |s| == 2
     ensures UInt16ToSeq(SeqToUInt16(s)) == s
   {}
 
-  method UInt16ToArray(x: UInt16) returns (ret: array<UInt8>)
+  method UInt16ToArray(x: uint16) returns (ret: array<uint8>)
     ensures fresh(ret)
     ensures UInt16ToSeq(x) == ret[..]
     ensures ret.Length == 2
   {
-    ret := new UInt8[2];
-    ret[0] := (x / 0x100) as UInt8;
-    ret[1] := (x % 0x100) as UInt8;
+    ret := new uint8[2];
+    ret[0] := (x / 0x100) as uint8;
+    ret[1] := (x % 0x100) as uint8;
   }
 
-  function method arrayToUInt16(p: array<UInt8>): (ret: UInt16)
-    reads p
-    requires p.Length == 2
-    ensures SeqToUInt16(p[..]) == ret
+  function method ArrayToUInt16(a: array<uint8>): (ret: uint16)
+    reads a
+    requires a.Length == 2
+    ensures SeqToUInt16(a[..]) == ret
   {
-    var x0 := p[0] as int * 0x100;
-    assert x0 <= 0x100 * 0x100;
-    var x := x0 + p[1] as int;
-    assert x < UINT16_LIMIT;
-    x as UInt16
+    var x0 := a[0] as int * 0x100;
+    var x := x0 + a[1] as int;
+    x as uint16
   }
 
-  function method UInt32ToSeq(x: UInt32): seq<UInt8>
+  function method UInt32ToSeq(x: uint32): seq<uint8>
     ensures |UInt32ToSeq(x)| == 4
   {
-    var b0 := ( x / 0x100_0000) as UInt8;
-    var x0: UInt32 := x - (b0 as UInt32 * 0x100_0000);
+    var b0 := ( x / 0x100_0000) as uint8;
+    var x0: uint32 := x - (b0 as uint32 * 0x100_0000);
 
-    var b1 := (x0 / 0x1_0000) as UInt8;
-    var x1: UInt32 := x0 - (b1 as UInt32 * 0x1_0000);
+    var b1 := (x0 / 0x1_0000) as uint8;
+    var x1: uint32 := x0 - (b1 as uint32 * 0x1_0000);
 
-    var b2 := (x1 / 0x100) as UInt8;
+    var b2 := (x1 / 0x100) as uint8;
 
-    var b3 := (x1 % 0x100) as UInt8;
+    var b3 := (x1 % 0x100) as uint8;
     [b0, b1, b2, b3]
   }
 
-  function method SeqToUInt32(p: seq<UInt8>): UInt32
-    requires |p| == 4
+  function method SeqToUInt32(s: seq<uint8>): uint32
+    requires |s| == 4
   {
-    var x0 := p[0] as int * 0x100_0000;
-    var x1 := x0 + p[1] as int * 0x1_0000;
-    var x2 := x1 + p[2] as int * 0x100;
-    var x := x2 + p[3] as int;
-    assert x < UINT32_LIMIT;
-    x as UInt32
+    var x0 := s[0] as int * 0x100_0000;
+    var x1 := x0 + s[1] as int * 0x1_0000;
+    var x2 := x1 + s[2] as int * 0x100;
+    var x := x2 + s[3] as int;
+    x as uint32
   }
 
-  lemma UInt32SeqSerDeser(x: UInt32)
+  lemma UInt32SeqSerDeser(x: uint32)
     ensures SeqToUInt32(UInt32ToSeq(x)) == x
   {}
 
-  lemma UInt32SeqDeserSer(s: seq<UInt8>)
+  lemma UInt32SeqDeserSer(s: seq<uint8>)
     requires |s| == 4
     ensures UInt32ToSeq(SeqToUInt32(s)) == s
   {}
 
-  method UInt32ToArray(x: UInt32) returns (ret: array<UInt8>)
+  method UInt32ToArray(x: uint32) returns (ret: array<uint8>)
     ensures fresh(ret)
     ensures UInt32ToSeq(x) == ret[..]
     ensures ret.Length == 4
   {
     var x' := x;
-    ret := new UInt8[4];
+    ret := new uint8[4];
 
-    ret[0] := (x' / 0x100_0000) as UInt8;
-    x' := x' - (ret[0] as UInt32 * 0x100_0000);
+    ret[0] := (x' / 0x100_0000) as uint8;
+    x' := x' - (ret[0] as uint32 * 0x100_0000);
 
-    ret[1] := (x' / 0x1_0000) as UInt8;
-    x' := x' - (ret[1] as UInt32 * 0x1_0000);
+    ret[1] := (x' / 0x1_0000) as uint8;
+    x' := x' - (ret[1] as uint32 * 0x1_0000);
 
-    ret[2] := (x' / 0x100) as UInt8;
+    ret[2] := (x' / 0x100) as uint8;
 
-    ret[3] := (x' % 0x100) as UInt8;
+    ret[3] := (x' % 0x100) as uint8;
   }
 
-  function method ArrayToUInt32(p: array<UInt8>): (ret: UInt32)
-    reads p
-    requires p.Length == 4
-    ensures SeqToUInt32(p[..]) == ret
+  function method ArrayToUInt32(a: array<uint8>): (ret: uint32)
+    reads a
+    requires a.Length == 4
+    ensures SeqToUInt32(a[..]) == ret
   {
-    var x0 := p[0] as int * 0x100_0000;
-    var x1 := x0 + p[1] as int * 0x1_0000;
-    var x2 := x1 + p[2] as int * 0x100;
-    var x := x2 + p[3] as int;
-    assert x < UINT32_LIMIT;
-    x as UInt32
+    var x0 := a[0] as int * 0x100_0000;
+    var x1 := x0 + a[1] as int * 0x1_0000;
+    var x2 := x1 + a[2] as int * 0x100;
+    var x := x2 + a[3] as int;
+    x as uint32
   }
 }
