src/SDK/Common.dfy
@@ -2,25 +2,24 @@ include "../StandardLibrary/StandardLibrary.dfy"
 include "../StandardLibrary/UInt.dfy"
 include "./AlgorithmSuite.dfy"
 
-
 module Materials {
   import opened StandardLibrary
   import opened UInt = StandardLibrary.UInt
   import AlgorithmSuite
 
-  type EncryptionContext = seq<(seq<UInt8>, seq<UInt8>)>
+  type EncryptionContext = seq<(seq<uint8>, seq<uint8>)>
 
   datatype EncryptedDataKey = EncryptedDataKey(providerID : string, 
-                                               providerInfo : seq<UInt8>,
-                                               ciphertext : seq<UInt8>)
+                                               providerInfo : seq<uint8>,
+                                               ciphertext : seq<uint8>)
 
   // TODO: Add keyring trace
   class EncryptionMaterials {
     var algorithmSuiteID: AlgorithmSuite.ID
     var encryptedDataKeys: seq<EncryptedDataKey>
     var encryptionContext: Option<EncryptionContext>
-    var plaintextDataKey: Option<seq<UInt8>>
-    var signingKey: Option<seq<UInt8>>
+    var plaintextDataKey: Option<seq<uint8>>
+    var signingKey: Option<seq<uint8>>
 
     predicate Valid() 
       reads this
@@ -32,8 +31,8 @@ module Materials {
     constructor(algorithmSuiteID: AlgorithmSuite.ID,
                 encryptedDataKeys: seq<EncryptedDataKey>, 
                 encryptionContext: Option<EncryptionContext>, 
-                plaintextDataKey: Option<seq<UInt8>>,
-                signingKey: Option<seq<UInt8>>)
+                plaintextDataKey: Option<seq<uint8>>,
+                signingKey: Option<seq<uint8>>)
       requires |encryptedDataKeys| > 0 ==> plaintextDataKey.Some?
       ensures Valid()
     {
@@ -44,7 +43,7 @@ module Materials {
       this.signingKey := signingKey;
     }
 
-    method SetPlaintextDataKey(dataKey: seq<UInt8>)
+    method SetPlaintextDataKey(dataKey: seq<uint8>)
       requires Valid()
       requires plaintextDataKey.None?
       modifies `plaintextDataKey
@@ -69,22 +68,22 @@ module Materials {
   class DecryptionMaterials {
     var algorithmSuiteID: AlgorithmSuite.ID
     var encryptionContext: Option<EncryptionContext>
-    var plaintextDataKey: Option<seq<UInt8>>
-    var verificationKey: Option<seq<UInt8>>
+    var plaintextDataKey: Option<seq<uint8>>
+    var verificationKey: Option<seq<uint8>>
     
     // TODO add Valid()
 
     constructor(algorithmSuiteID: AlgorithmSuite.ID,
                 encryptionContext: Option<EncryptionContext>,
-                plaintextDataKey: Option<seq<UInt8>>,
-                verificationKey: Option<seq<UInt8>>) {
+                plaintextDataKey: Option<seq<uint8>>,
+                verificationKey: Option<seq<uint8>>) {
       this.algorithmSuiteID := algorithmSuiteID;
       this.encryptionContext := encryptionContext;
       this.plaintextDataKey := plaintextDataKey;
       this.verificationKey := verificationKey;
     }
 
-    method setPlaintextDataKey(dataKey: seq<UInt8>)
+    method setPlaintextDataKey(dataKey: seq<uint8>)
       requires plaintextDataKey.None?
       modifies `plaintextDataKey
       ensures plaintextDataKey == Some(dataKey)
@@ -109,13 +108,13 @@ module Materials {
 
     }
     
-    function method memcmp_le (a : seq<UInt8>, b : seq<UInt8>, len : nat) : (res : Option<bool>)
+    function method memcmp_le (a : seq<uint8>, b : seq<uint8>, len : nat) : (res : Option<bool>)
         requires |a| >= len
         requires |b| >= len {
         if len == 0 then None else if a[0] != b[0] then Some(a[0] < b[0]) else memcmp_le (a[1..], b[1..], len - 1)
     }
 
-    predicate method lex_lt(b : seq<UInt8>, a : seq<UInt8>)
+    predicate method lex_lt(b : seq<uint8>, a : seq<uint8>)
     {
         match memcmp_le(a,b, if |a| < |b| then |a| else |b|) {
         case Some(b) => !b
@@ -123,27 +122,27 @@ module Materials {
         }
   }
 
-    predicate method lt_keys(b : (seq<UInt8>, seq<UInt8>), a : (seq<UInt8>, seq<UInt8>)) {
+    predicate method lt_keys(b : (seq<uint8>, seq<uint8>), a : (seq<uint8>, seq<uint8>)) {
         lex_lt(b.0, a.0)
     }
 
-    function method EncCtxFlatten (x : seq<(seq<UInt8>, seq<UInt8>)>) : seq<UInt8> { 
+    function method EncCtxFlatten (x : seq<(seq<uint8>, seq<uint8>)>) : seq<uint8> { 
         if x == [] then [] else
         x[0].0 + x[0].1 + EncCtxFlatten(x[1..])
     }
 
-    function method FlattenSortEncCtx(x : seq<(seq<UInt8>, seq<UInt8>)>) : seq<UInt8>
+    function method FlattenSortEncCtx(x : seq<(seq<uint8>, seq<uint8>)>) : seq<uint8>
     {
         EncCtxFlatten(naive_merge_sort(x, lt_keys))
     }
 
-    function method enc_ctx_lookup(x : seq<(seq<UInt8>, seq<UInt8>)>, k : seq<UInt8>) : Option<seq<UInt8>>
+    function method enc_ctx_lookup(x : seq<(seq<uint8>, seq<uint8>)>, k : seq<uint8>) : Option<seq<uint8>>
     {
         if |x| == 0 then None else
         if x[0].0 == k then Some(x[0].1) else enc_ctx_lookup(x[1..], k)
     }
 
-    function method enc_ctx_of_strings(x : seq<(string, string)>) : seq<(seq<UInt8>, seq<UInt8>)>  {
+    function method enc_ctx_of_strings(x : seq<(string, string)>) : seq<(seq<uint8>, seq<uint8>)>  {
         if x == [] then [] else
         [(byteseq_of_string_lossy(x[0].0), byteseq_of_string_lossy(x[0].1))] + enc_ctx_of_strings(x[1..])
     }
